prove ReprAfterSubstituteCompactReplacementInduction1. Yet to prove subtheorem dependecies

Splinter/Betree/LinkedBetree.i.dfy
@@ -704,8 +704,9 @@ module LinkedBetreeMod
     }
 
     // Returns the address of all the nodes on the path, from root up to and including target
-    function AddrsOnPath() : set<Address> 
+    function AddrsOnPath() : (out: set<Address>)
       requires Valid()
+      ensures forall addr | addr in out :: addr in linked.diskView.entries
       decreases depth
     {
       if depth == 0 then {linked.root.value}
